Henry \cite{Henry60} assumed that a ``representative average of the value of the diffusion
coefficient, $D$, could be found and used as a constant scalar throughout the field of flow without
distorting the essential features of the problem.'' Additionally, Henry assumed the Bousinesq
approximation, which implies the existence of a stream function, defined as 

\begin{equation*}
    u'=\pderiv{\psi'}{y'},\; v'=-\pderiv{\psi'}{x'} 
\end{equation*} 

Thus, using these assumptions allows one to write the steady state transport equations in the
following dimensionless form 
\begin{align} 
  &a\left( \frac{\partial^2 \psi}{\partial x^2} + \frac{\partial^2 \psi}{\psi y^2} \right) =
    \frac{\partial C}{\partial x} + \frac{1}{\xi}, \label{eqn:Streamfunction}\\
  &b\left( \frac{\partial^2 C}{\partial x^2} + \frac{\partial^2 C}{\psi y^2} \right) =
    \frac{\partial \psi}{\partial y}\frac{\partial C}{\partial x} 
    - \frac{\partial \psi}{\partial x}\frac{\partial C}{\partial y} 
    + \frac{1}{\xi}\frac{\partial \psi}{\partial y} + \frac{\partial C}{\partial x} +
    \frac{1}{\xi}, \label{eqn:Concentration}
\end{align}
where $\psi$ is the dimensionless stream function, $C$ is the dimensionless concentration,
$\xi=\frac{L}{d}$ is the aspect ratio of the problem domain. Additionally, the dimensionless
parameters $a$ and $b$ are given by
\begin{equation} \label{eqn:ab}
  a =\frac{Q}{k_1 d} \text{ and } b = \frac{D}{Q} 
\end{equation}
where $Q$ is the freshwater recharge, $k_1$ is related to the hydraulic conductivity, $K$, by $k_1 =
K\left( \frac{\rho_s - \rho_0}{\rho_0} \right)$, with $\rho_0$ and $\rho_s$ the freshwater and
seawater densities, respectively.

Henry used the boundary conditions 
\begin{equation} \label{eqn:BC)} \begin{array}{lcr} 
    \psi = 0, \pderiv{c}{y} =0 \spbox{at} y=0
    & \qquad
    & \pderiv{\psi}{x} = 0, c = 0 \spbox{at} x=0 \\
    \psi= 1, \pderiv{c}{y} = 0 \spbox{at} y=1
    & \qquad
    & \pderiv{\psi}{x} =0,  c=1 \spbox{at} x=\xi 
\end{array} \end{equation}
and what he termed as Fourier-Galerkin method, whereby one substitutes
\begin{align}
  \psi = \sum_{m=1}^{\infty}\sum_{n=0}^{\infty} A_{m,n} \sin{m\pi y} \cos{n\pi\frac{x}{\xi}}
    \label{eqn:psi} \\
  C = \sum_{r=0}^{\infty}\sum_{s=1}^{\infty} B_{r,s} \cos{r\pi y} \sin{s\pi\frac{x}{\xi}}
    \label{eqn:C}
\end{align}
into \eqref{eqn:Streamfunction} and \eqref{eqn:Concentration}, then multiplying
\eqref{eqn:Streamfunction} by $4 \sin\left(g \pi y\right) \cdot \cos\left(h \pi \frac{x}{\xi}\right)$ and
\eqref{eqn:Concentration} by $4 \cos\left(g \pi y\right)\cdot \sin\left(h \pi \frac{x}{\xi}\right)$ to obtain
\begin{align}
    \varepsilon(h)\cdot a \pi^{2} A_{g,h} \left(g^{2} + \frac{h^{2} }{\xi ^{2} } \right) \xi 
      &= \sum _{r=0}^{\infty} B_{r,h} \cdot h \cdot N \left(g,r\right) 
      + \frac{4}{\pi} W \left(g, h\right) \label{eqn:A}\\
    \varepsilon(g) \cdot b \pi ^{2} B_{g,h} \left(g^{2} + \frac{h^{2}}{\xi ^{2}}\right) \xi 
      &= \frac{\pi }{4} 
      \sum _{m=1}^{\infty } \sum _{n=0}^{\infty } \sum_{r=0}^{\infty } \sum _{s=1}^{\infty}
      A_{m,n} B_{r,s} (msLR - nrFG) \nonumber \\
      & + \sum_{n=0}^{\infty} A_{g,n} \cdot g \cdot N(h, n) 
      + \varepsilon(g) \cdot \sum_{s=1}^{\infty} B_{g,s} \cdot s\cdot N(h, s) 
      \nonumber \\ 
      &+ \frac{4}{\pi} W(g,h) \label{eqn:B}
\end{align}
where
\begin{equation*}
  \varepsilon(g) = \begin{cases} 2 & \text{if } g=0 \\
    1 & \text{if } g \ne 0
  \end{cases}
\end{equation*}
\begin{equation*}
  N(h,n) = \frac{\left( -1 \right)^{h+n}-1}{h+n} + \frac{\left( -1 \right)^{h-n}-1}{h-n},
\end{equation*}
\begin{equation*}
  W(h,n) = \begin{cases} \frac{\left( -1 \right)^h -1}{h} &\text{if } g = 0 \\
    0& \text{if } g\ne 0
  \end{cases}
\end{equation*}
\begin{align*}
  F &= \delta_{(m-r),g} + \delta_{(r-m),g} - \delta_{(m+r),q}, \\
  L &= \delta_{(m-r),g} + \delta_{(r-m),g} + \delta_{(m+r),q},
\end{align*}
\begin{equation*}
  G = \frac{\left( -1 \right)^{h+n-s}-1}{h+n-s} 
    + \frac{\left( -1 \right)^{h-n+s}-1}{h-n+s}
    - \frac{\left( -1 \right)^{h+n+s}-1}{h+n+s}
    + \frac{\left( -1 \right)^{h-n-s}-1}{h-n-s},
\end{equation*}
\begin{equation*}
  R = \frac{\left( -1 \right)^{h+n-s}-1}{h+n-s} 
    + \frac{\left( -1 \right)^{h-n+s}-1}{h-n+s}
    + \frac{\left( -1 \right)^{h+n+s}-1}{h+n+s}
    + \frac{\left( -1 \right)^{h-n-s}-1}{h-n-s},
\end{equation*}
and $\delta_{i,j}$ is the Kronecker delta such that
\begin{equation*}
  \delta_{i,j} = \begin{cases} 1 & \text{if } i=j \\
    0 & \text{if } i\ne j
  \end{cases}
\end{equation*}
